spinlock_atomic/LockIA.v
@@ -7,101 +7,91 @@ Module LockIA. Section LockIA.
   Import LockAS.
   Context `{!crisG Γ Σ α β τ _S _I, !memG, !schG, !spinlockG}.
 
+  Context (E : coPset).
+  Context (LockInE: ↑N_SpinLockA ⊆ E).  
+  
   Definition init_cond : iProp Σ := emp%I.
 
   Local Definition MemP := MemP.t.
   Local Definition SpinLockA := SpinLockA.t.
   Local Definition SpinLockI := SpinLockI.t.
-  Local Definition IstFull := (IstProd (IstSB (Mod.scopes SpinLockA) IstTrue) IstEq).
-  Local Notation MA := (SpinLockA ★ MemP).
+  Local Definition IstFull := (IstProd (IstSB (Mod.scopes (SpinLockA E)) IstTrue) IstEq).
+  Local Notation MA := (SpinLockA E ★ MemP).
   Local Notation MI := (SpinLockI ★ MemP).
 
   Lemma newlock_simF :
     ISim.sim_fun open MA MI init_cond IstFull (Some SpinLockHdr.newlock).
   Proof.
     init_simF.
+    steps_l; unfold_real_lat_l.
 
-    (* preprocess initial conditions *)
-    steps_l. steps_r.
-
-    destruct (arg↓) as [v|] eqn:E; cycle 1.
+    destruct (arg↓) as [v|] eqn: EQ; cycle 1.
     { sch_yield_l. steps_l. force_l (tt↑). steps_l.
       ru_l False%I. iSplitL; cycle 1.
       { iIntros "F". iExFalso. et. }
       iIntros ([]) "[_ [[% _] _]]"; subst; hss.
     }
-
-    (* tgt yield *)
-    steps_r.
-    sch_yield_rr.
+    steps_r. sch_yield_rr.
 
     (* tgt inline - mem alloc *)
-    steps_r. inline_r. steps_r. force_r 1.
+    steps_r. inline_r. steps_r.
+    unfold_real_lat_r. force_r 1.
     iSplit; et. iIntros "[%blk [-> [↦ _]]]".
     steps_r; hss_r; steps_r.
-
-    (* tgt yield *)
     sch_yield_rr.
 
     (* tgt inline - mem store *)
-    steps_r. inline_r. steps_r. force_r (blk, 0%Z, _, _); s.
+    steps_r. inline_r. steps_r.
+    unfold_real_lat_r. force_r (blk, 0%Z, _, _); s.
     iFrame "↦". iSplit; try done. iIntros "[↦ ->]".
     steps_r; hss_r; steps_r.
 
     (* src/tgt yield *)
-    sch_yield_rr.
-    sch_yield_l; steps_l.
+    sch_yield_rr. sch_yield_l; steps_l.
 
     (* lock token allocation *)
     iMod (own_alloc (Excl ())) as "[%γ TKN]"; [done|].
-
     force_l ((Vptr (blk, 0%Z))↑). steps_l.
     ru_l emp%I.
-    iSplitL "↦ TKN"; cycle 1.
+    iSplitR "IST"; cycle 1.
     { iIntros "_". steps_l. sch_yield_l. step. iSplit; done. }
-    { iIntros ([n P]) "[W [[_ P] _]]"; s.
-      iSplitR; [eauto|].
-      unfold_pre_post. iRevert "W".
-      iApply (winv_fupd (S n)).
-      iMod (inv_alloc (LockAS.lock_inv (blk, 0%Z) P γ) _ _ _ N_SpinLockA
-        with "[↦ P TKN]") as "#I"; ss.
-      { rewrite /lock_inv; SL_red; iRight; iFrame. }
-      iModIntro; iFrame. iSplit; eauto. iExists _, _; iSplit; eauto.
-      rewrite /is_lock; iExists _; iFrame "I"; done.
-      Unshelve. all: exact 0.
-    }
+    iIntros ([n P]) "[W [[_ P] _]]"; s.
+    iSplitR; [eauto|].
+    unfold_pre_post. iRevert "W".
+    iApply (winv_fupd (S n)).
+    iMod (inv_alloc (LockAS.lock_inv (blk, 0%Z) P γ) _ _ _ N_SpinLockA
+      with "[↦ P TKN]") as "#I"; ss.
+    { rewrite /lock_inv; SL_red; iRight; iFrame. }
+    iModIntro; iFrame. iSplit; eauto. iExists _, _; iSplit; eauto.
+    rewrite /is_lock; iExists _; iFrame "I"; done.
+    Unshelve. all: exact 0.
   (*SLOW*)Qed.
 
   Lemma acquire_simF : ISim.sim_fun open MA MI init_cond IstFull (Some SpinLockHdr.acquire).
   Proof.
     init_simF.
-
-    (* process src precondition *)
-    steps_l. steps_r.
+    steps_l; unfold_real_lat_l.
 
     (* ill-formed argument *)
     destruct (arg↓) as [l|] eqn : Heqarg; cycle 1.
-    { rewrite /real_peek. unfold_iter_l. steps_l.
-      sch_yield_l. steps_l. force_l false. steps_l.
-      force_l (tt↑). steps_l.
+    { sch_yield_l. steps_l. force_l false. force_l (tt↑). steps_l.
       ru_l False%I. iSplitL; cycle 1.
       { iIntros "F". iExFalso. et. }
       iIntros ([[] []]) "[_ [[% _] _]]"; subst; hss.
     }
     destruct (or_else (pargs [Tptr] l) (0, 0%Z)) as [blk ofs] eqn: EQ.
+    hss. steps_r.
 
-    steps_r. rewrite /real_peek.
-    unfold_iter_l; steps_l. unfold_iter_r. steps_r.
     (* start coinduction for lock acquire/failure *)
     iApply wsim_reset. iStopProof.
-    revert st_src. combine_quant st_tgt.
+    revert st_tgt. combine_quant st_src.
     eapply wsim_coind.
-    iIntros (g' _ CIH [st_tgt st_src]) "IST /=".
+    iIntros (g' _ CIH [st_src st_tgt]) "IST /=".
     destruct_quant CIH.
 
-    sch_yield_rr.
-    sch_yield_l; steps_l.
+    unfold_iter_r. steps_r. sch_yield_rr. sch_yield_l; steps_l.
     steps_r. inline_r. steps_r.
+    unfold_real_lat_r.
     ru_r. iIntros (pr) "UPD". rename _q into ret.
 
     destruct (classic (ret = (Vint 0)↑)).
@@ -129,7 +119,6 @@ Module LockIA. Section LockIA.
       sch_yield_l.
       step. et.
     }
-    
     { force_l true. steps_l.
       ru_l (⌜ret = (Vint 1)↑⌝ ∗ Own pr)%I.
       iSplitL "UPD".
@@ -149,10 +138,9 @@ Module LockIA. Section LockIA.
         iExists _; iFrame "I"; done.
       }
       iIntros "[-> PR]".
-      steps_l. unfold_iter_l. steps_l.
+      steps_l. unfold_real_lat_l.
       force_r; iFrame. steps_r. hss. steps_r.
       do 2 sch_yield_rr. steps_r.
-      unfold_iter_r. steps_r.
       by_coind CIH. iFrame.
     }
   Unshelve. all: try exact 1%Qp; try exact (Vint 0); eauto.
@@ -161,8 +149,7 @@ Module LockIA. Section LockIA.
   Lemma release_simF : ISim.sim_fun open MA MI init_cond IstFull (Some SpinLockHdr.release).
   Proof.
     init_simF.
-    (* process src precondition *)
-    steps_l. steps_r.
+    steps_l; unfold_real_lat_l.
 
     (* ill-formed argument *)
     destruct (arg↓) as [l|] eqn : Heqarg; cycle 1.
@@ -171,11 +158,11 @@ Module LockIA. Section LockIA.
       { iIntros "F". iExFalso. et. }
       iIntros ([[] []]) "[_ [[% _] _]]"; subst; hss.
     }
-    
     destruct (or_else (pargs [Tptr] l) (0, 0%Z)) as [blk ofs] eqn: EQ.
-    steps_r.
-    sch_yield_rr.
+
+    steps_r. sch_yield_rr.
     steps_r. inline_r. steps_r.
+    unfold_real_lat_r.
     ru_r. iIntros (pr) "UPD". rename _q into ret.
     sch_yield_l; steps_l. force_l (Vundef↑). steps_l.
     ru_l (⌜ret = (Vint 0)↑⌝ ∗ Own pr)%I.
@@ -211,7 +198,7 @@ Module LockIA. Section LockIA.
   (* ctxr works as a unit in compositions of module simulations *)
   Lemma ctxr :
     ctx_refines
-      (SpinLockA.t ★ MemP.t, emp%I)
+      (SpinLockA.t E ★ MemP.t, emp%I)
       (SpinLockI.t ★ MemP.t, emp%I).
   Proof. eapply main_adequacy, sim; eauto. Qed.
 End LockIA. End LockIA.
