incr/FaaIA.v
@@ -6,8 +6,8 @@ Module FaaIA. Section FaaIA.
   Context `{!crisG Γ Σ α β τ _S _I, !memG, !schG}.
 
   Local Definition IstFull := (IstProd (IstSB FaaA.t.(Mod.scopes) IstTrue) IstEq).
-  Local Definition MA := (FaaA.t ★ MemA.t).
-  Local Definition MI := (FaaI.t ★ MemA.t).
+  Local Definition MA := (FaaA.t ★ MemP.t).
+  Local Definition MI := (FaaI.t ★ MemP.t).
 
   Lemma faa2_simF : ISim.sim_fun open MA MI True%I IstFull (Some FaaHdr.faa2).
   Proof.
@@ -23,23 +23,27 @@ Module FaaIA. Section FaaIA.
     sch_yield_l; steps_l. rename _q into v.
 
     rewrite /MemHdr.faa; steps_r; inline_r.
-    force_r (_, _, _, Vint v); forces_r; iFrame "ASM"; iSplit; eauto.
-    steps_r; iDestruct "GRT" as "[[PT ->] ->]"; hss_r.
-    steps_r; inline_r.
-    force_r (_, _, _, _); forces_r; iFrame "PT"; iSplit; eauto.
-    steps_r; iDestruct "GRT" as "[[PT ->] ->]"; hss_r. steps_r.
+    unfold_real_lat_r. force_r (_, _, _, Vint v).
+    iFrame "ASM". iSplit; et.
+    iIntros "[PT ->]". steps_r. hss_r. steps_r.
+    
+    inline_r.
+    unfold_real_lat_r. force_r (_, _, _, _).
+    iFrame "PT". iSplit; et.
+    iIntros "[PT ->]". steps_r. hss_r. steps_r.
 
     force_l; iFrame "PT"; steps_l.
-
     sch_yield_rr.
     Unshelve. all: try exact 0.
     sch_yield_l; steps_l; clear v; rename _q into v.
     steps_r; inline_r.
-    force_r (_, _, _, _); forces_r; iFrame "ASM"; iSplit; eauto.
-    steps_r; iDestruct "GRT" as "[[PT ->] ->]"; hss_r.
+    unfold_real_lat_r. force_r (_, _, _, _).
+    iFrame. iSplit; et.
+    iIntros "[PT ->]". steps_r. hss_r. steps_r.
     steps_r; inline_r.
-    force_r (_, _, _, _); forces_r; iFrame "PT"; iSplit; eauto.
-    steps_r; iDestruct "GRT" as "[[PT ->] ->]"; hss_r.
+    unfold_real_lat_r. force_r (_, _, _, _).
+    iFrame. iSplit; et.
+    iIntros "[PT ->]". steps_r. hss_r. steps_r.
 
     force_l; iFrame "PT"; steps_l.
     steps_r.
