increment/IncrementIAproof.v
@@ -7,8 +7,8 @@ Module IncrementIA. Section IncrementIA.
   Context `{!crisG Γ Σ α β τ _S _I, !memG, !schG}.
 
   Local Definition IstFull := (IstProd (IstSB IncrementA.t.(Mod.scopes) IstTrue) IstEq).
-  Local Definition MA := (IncrementA.t ★ MemA.t).
-  Local Definition MI := (IncrementI.t ★ MemA.t).
+  Local Definition MA := (IncrementA.t ★ MemP.t).
+  Local Definition MI := (IncrementI.t ★ MemP.t).
 
   Lemma increment_simF : ISim.sim_fun open MA MI True%I IstFull (Some IncrementHdr.increment).
   Proof.
@@ -23,7 +23,7 @@ Module IncrementIA. Section IncrementIA.
     norm_l. norm_r.
 
     iApply wsim_reset.
-    iStopProof. revert st_src1. combine_quant st_tgt1.
+    iStopProof. revert st_src. combine_quant st_tgt.
     eapply wsim_coind.
     iIntros (g' _ CIH [st_t st_s]) "%GG' /=".
     destruct_quant CIH.
@@ -35,9 +35,9 @@ Module IncrementIA. Section IncrementIA.
 
     sch_yield_l. steps_l. rename _q into v.
 
-    steps_r. inline_r. force_r (blk, ofs, 1%Qp, Vint v). steps_r.
-    forces_r. iFrame "ASM". iSplit; eauto.
-    steps_r. iDestruct "GRT" as "[[PT ->] ->]". hss_r. steps_r.
+    steps_r. inline_r. unfold_real_lat_r. force_r (blk, ofs, 1%Qp, Vint v).
+    iFrame. iSplit; et.
+    iIntros "[PT ->]". steps_r. hss_r. steps_r.
 
     force_l false. steps_l. force_l; iFrame "PT". steps_l. sch_yield_l. steps_l.
     unfold_iterC_l. steps_l.
@@ -46,12 +46,11 @@ Module IncrementIA. Section IncrementIA.
     sch_yield_rr. steps_r.
 
     sch_yield_l. steps_l. rename _q into v'.
-    inline_r. force_r (_, _, _, _, _, _, _, _, _, _). forces_r. iFrame "ASM".
-    iSplitL ""; eauto.
-    { iSplit; eauto. iSplit; [iPureIntro; split; [refl|ss]|ss]. des_ifs. }
-    Unshelve. all: try exact 0; try exact 1%Qp; try exact (Vint 0).
+    inline_r. unfold_real_lat_r. force_r (_, _, _, _, _, _, _, _, _, _).
+    iSplitL "ASM".
+    { s. iFrame. repeat (iSplit; eauto). s. des_ifs. }
+    iIntros "[-> [GRT _]]". steps_r. hss. steps_r.
 
-    steps_r. iDestruct "GRT" as "[[-> [GRT _]] ->]". hss_r. steps_r.
     destruct (dec v' v) as [?|Heq]; [subst; ss|ss].
     { force_l true. steps_l. force_l; iFrame "GRT"; steps_l.
       sch_yield_rr. steps_r.
@@ -70,6 +69,6 @@ Module IncrementIA. Section IncrementIA.
       iApply wsim_progress. iApply wsim_base.
       iIntros "?". iApply (CIH). iFrame.
     }
-    Unshelve. all: eauto.
+    Unshelve. all: eauto. all: try exact 1%Qp. all: try exact Vundef.
   (*SLOW*)Qed.
 End IncrementIA. End IncrementIA.
